tests/VersoBlueprintTests/BlueprintImportedContributions/FacetDoc.lean
@@ -1,0 +1,17 @@
+/-
+Copyright (c) 2026 Lean FRO LLC. All rights reserved.
+Released under Apache 2.0 license as described in the file LICENSE.
+Author: Emilio J. Gallego Arias
+-/
+import VersoBlueprintTests.BlueprintImportedContributions.FacetStatement
+import VersoBlueprintTests.BlueprintImportedContributions.FacetProof
+
+open Verso.Genre
+
+#doc (Manual) "Completed facets" =>
+
+{include 0 VersoBlueprintTests.BlueprintImportedContributions.FacetPlaceholder}
+{include 0 VersoBlueprintTests.BlueprintImportedContributions.FacetStatement}
+{include 0 VersoBlueprintTests.BlueprintImportedContributions.FacetProof}
+
+{blueprint_graph}
