tests/VersoBlueprintTests/BlueprintImportedContributions/FacetProof.lean
@@ -1,0 +1,20 @@
+/-
+Copyright (c) 2026 Lean FRO LLC. All rights reserved.
+Released under Apache 2.0 license as described in the file LICENSE.
+Author: Emilio J. Gallego Arias
+-/
+import VersoBlueprintTests.BlueprintImportedContributions.FacetPlaceholder
+
+open Verso.Genre Informal
+
+#doc (Manual) "Proof source chapter" =>
+
+:::proof "filled_facet"
+%%%
+source := {
+  document := "facet-proof-paper"
+  spans := #[{ page := "2", pdf := some { path := "source/page-2.pdf" } }]
+}
+%%%
+A completed proof from page two.
+:::
